src/classes/SMT_classes_instances.v
@@ -15,46 +15,19 @@ From Stdlib Require Import Uint63.
 Require Import State BVList FArray.
 Require Export SMT_classes.
 
-Section StrictOrder.
-
-  Global Instance StrictOrder_to_OrdType {T : Type} {R : relation T}:
-    StrictOrder R -> OrdType T.
-  Proof.
-    split with R.
-    - apply StrictOrder_Transitive.
-    - intros ? y ? ->.
-      now apply StrictOrder_Irreflexive with y.
-  Defined.
-
-End StrictOrder.
 
 Section Unit.
   Let eqb : unit -> unit -> bool := fun _ _ => true.
-
-  Let lt : unit -> unit -> Prop := fun _ _ => False.
-
-  Global Instance unit_ord : OrdType unit.
-  Proof. exists lt; unfold lt; trivial.
-    intros; contradict H; trivial.
-  Defined.
 
   Global Instance unit_eqbtype : EqbType unit.
   Proof.
     exists eqb. intros. destruct x, y. unfold eqb. split; trivial.
   Defined.
 
-  Global Instance unit_comp : @Comparable unit unit_ord.
-  Proof.
-    split. intros. destruct x, y.
-    apply OrderedType.EQ; trivial.
-  Defined.
-
   Global Instance unit_inh : Inhabited unit := {| default_value := tt |}.
 
   Global Instance unit_compdec : CompDec unit := {|
     Eqb := unit_eqbtype;
-    Ordered := unit_ord;
-    Comp := unit_comp;
     Inh := unit_inh
   |}.
 
@@ -65,37 +38,6 @@ End Unit.
 
 Section Bool.
 
-  Definition ltb_bool x y := negb x && y.
-
-  Definition lt_bool x y := ltb_bool x y = true.
-
-  Global Instance bool_ord : OrdType bool.
-  Proof.
-    exists lt_bool.
-    intros x y z.
-    case x; case y; case z; intros; simpl; subst; auto.
-    intros x y.
-    case x; case y; intros; simpl in H; easy.
-  Defined.
-
-  Global Instance bool_comp: Comparable bool.
-  Proof.
-    constructor.
-    intros x y.
-    case_eq (ltb_bool x y).
-    intros.
-    apply OrderedType.LT.
-    unfold lt, bool_ord, lt_bool. auto.
-    case_eq (Bool.eqb x y).
-    intros.
-    apply OrderedType.EQ.
-    apply Bool.eqb_prop. auto.
-    intros.
-    apply OrderedType.GT.
-    unfold lt, bool_ord, lt_bool. auto.
-    case x in *; case y in *; auto.
-  Defined.
-
   Global Instance bool_eqbtype : EqbType bool :=
     {| eqb := Bool.eqb; eqb_spec := eqb_true_iff |}.
 
@@ -105,58 +47,28 @@ Section Bool.
 
   Global Instance bool_compdec : CompDec bool := {|
     Eqb := bool_eqbtype;
-    Ordered := bool_ord;
-    Comp := bool_comp;
     Inh := bool_inh
   |}.
-
-
-  Lemma ltb_bool_iff_lt: forall x y, ltb_bool x y = true <-> lt_bool x y.
-  Proof. intros x y; split; intro H;
-         case_eq x; case_eq y; intros; subst; compute in *; easy.
-  Qed.
 
 End Bool.
 
 
 Section Z.
 
-  Global Instance Z_ord : OrdType Z.
-  Proof.
-    exists Z_as_OT.lt.
-    exact Z_as_OT.lt_trans.
-    exact Z_as_OT.lt_not_eq.
-  Defined.
-
-
-  Global Instance Z_comp: Comparable Z.
-  Proof.
-    constructor.
-    apply Z_as_OT.compare.
-  Defined.
-
   Global Instance Z_eqbtype : EqbType Z :=
     {| eqb := Z.eqb; eqb_spec := Z.eqb_eq |}.
 
   Global Instance Z_dec : DecType Z := @EqbToDecType _ Z_eqbtype.
 
-
   Global Instance Z_inh : Inhabited Z := {| default_value := 0%Z |}.
-
 
   Global Instance Z_compdec : CompDec Z := {|
     Eqb := Z_eqbtype;
-    Ordered := Z_ord;
-    Comp := Z_comp;
     Inh := Z_inh
   |}.
 
   (** lt and eq predicates in Prop and their equivalences with the ones in bool *)
   Definition eqP_Z x y := if Z.eqb x y then True else False.
-  Definition ltP_Z x y := if Z.ltb x y then True else False.
-  Definition leP_Z x y := if Z.leb x y then True else False.
-  Definition gtP_Z x y := if Z.gtb x y then True else False.
-  Definition geP_Z x y := if Z.geb x y then True else False.
 
   Lemma eq_Z_B2P: forall x y, Z.eqb x y = true <-> eqP_Z x y.
   Proof. intros x y; split; intro H.
@@ -164,76 +76,6 @@ Section Z.
          unfold eqP_Z in H.
          case_eq ((x =? y)%Z ); intros; try now subst.
          rewrite H0 in H. now contradict H.
-  Qed.
-
-  Lemma lt_Z_B2P: forall x y, Z.ltb x y = true <-> ltP_Z x y.
-  Proof. intros x y; split; intro H.
-         unfold ltP_Z; now rewrite H.
-         unfold ltP_Z in H.
-         case_eq ((x <? y)%Z ); intros; try now subst.
-         rewrite H0 in H. now contradict H.
-  Qed.
-
-  Lemma le_Z_B2P: forall x y, Z.leb x y = true <-> leP_Z x y.
-  Proof. intros x y; split; intro H.
-         unfold leP_Z; now rewrite H.
-         unfold leP_Z in H.
-         case_eq ((x <=? y)%Z ); intros; try now subst.
-         rewrite H0 in H. now contradict H.
-  Qed.
-
-  Lemma gt_Z_B2P: forall x y, Z.gtb x y = true <-> gtP_Z x y.
-  Proof. intros x y; split; intro H.
-         unfold gtP_Z; now rewrite H.
-         unfold gtP_Z in H.
-         case_eq ((x >? y)%Z ); intros; try now subst.
-         rewrite H0 in H. now contradict H.
-  Qed.
-
-  Lemma ge_Z_B2P: forall x y, Z.geb x y = true <-> geP_Z x y.
-  Proof. intros x y; split; intro H.
-         unfold geP_Z; now rewrite H.
-         unfold geP_Z in H.
-         case_eq ((x >=? y)%Z ); intros; try now subst.
-         rewrite H0 in H. now contradict H.
-  Qed.
-
-  Lemma lt_Z_B2P': forall x y, ltP_Z x y <-> Z.lt x y.
-  Proof. intros x y; split; intro H.
-         unfold ltP_Z in H.
-         case_eq ((x <? y)%Z ); intros; rewrite H0 in H; try easy.
-         now apply Z.ltb_lt in H0.
-         apply lt_Z_B2P.
-         now apply Z.ltb_lt.
-  Qed.
-
-  Lemma le_Z_B2P': forall x y, leP_Z x y <-> Z.le x y.
-  Proof. intros x y; split; intro H.
-         unfold leP_Z in H.
-         case_eq ((x <=? y)%Z ); intros; rewrite H0 in H; try easy.
-         now apply Z.leb_le in H0.
-         apply le_Z_B2P.
-         now apply Z.leb_le.
-  Qed.
-
-  Lemma gt_Z_B2P': forall x y, gtP_Z x y <-> Z.gt x y.
-  Proof. intros x y; split; intro H.
-         unfold gtP_Z in H.
-         case_eq ((x >? y)%Z ); intros; rewrite H0 in H; try easy.
-         now apply Zgt_is_gt_bool in H0.
-         apply gt_Z_B2P.
-         now apply Zgt_is_gt_bool.
-  Qed.
-
-  Lemma ge_Z_B2P': forall x y, geP_Z x y <-> Z.ge x y.
-  Proof. intros x y; split; intro H.
-         unfold geP_Z in H.
-         case_eq ((x >=? y)%Z ); intros; rewrite H0 in H; try easy.
-         rewrite Z.geb_leb in H0. rewrite le_Z_B2P in H0.
-         apply le_Z_B2P' in H0. now apply Z.ge_le_iff.
-         apply ge_Z_B2P.
-         rewrite Z.geb_leb. rewrite le_Z_B2P.
-         apply le_Z_B2P'. now apply Z.ge_le_iff.
   Qed.
 
   Lemma leibniz_eq_Z_B2P: forall x y, eqP_Z x y <-> Logic.eq x y.
@@ -248,34 +90,15 @@ End Z.
 
 Section Nat.
 
-  Global Instance Nat_ord : OrdType nat.
-  Proof.
-
-    exists Nat_as_OT.lt.
-    exact Nat_as_OT.lt_trans.
-    exact Nat_as_OT.lt_not_eq.
-  Defined.
-
-
-  Global Instance Nat_comp: Comparable nat.
-  Proof.
-    constructor.
-    apply Nat_as_OT.compare.
-  Defined.
-
   Global Instance Nat_eqbtype : EqbType nat :=
     {| eqb := Nat.eqb; eqb_spec := Nat.eqb_eq |}.
 
   Global Instance Nat_dec : DecType nat := EqbToDecType.
 
-
   Global Instance Nat_inh : Inhabited nat := {| default_value := O%nat |}.
-
 
   Global Instance Nat_compdec : CompDec nat := {|
     Eqb := Nat_eqbtype;
-    Ordered := Nat_ord;
-    Comp := Nat_comp;
     Inh := Nat_inh
   |}.
 
@@ -283,19 +106,6 @@ End Nat.
 
 
 Section Positive.
-
-  Global Instance Positive_ord : OrdType positive.
-  Proof.
-    exists Positive_as_OT.lt.
-    exact Positive_as_OT.lt_trans.
-    exact Positive_as_OT.lt_not_eq.
-  Defined.
-
-  Global Instance Positive_comp: Comparable positive.
-  Proof.
-    constructor.
-    apply Positive_as_OT.compare.
-  Defined.
 
   Global Instance Positive_eqbtype : EqbType positive :=
     {| eqb := Pos.eqb; eqb_spec := Pos.eqb_eq |}.
@@ -306,29 +116,13 @@ Section Positive.
 
   Global Instance Positive_compdec : CompDec positive := {|
     Eqb := Positive_eqbtype;
-    Ordered := Positive_ord;
-    Comp := Positive_comp;
     Inh := Positive_inh
   |}.
-
 
 End Positive.
 
 
 Section N.
-
-  Global Instance N_ord : OrdType N.
-  Proof.
-    exists N_as_OT.lt.
-    exact N_as_OT.lt_trans.
-    exact N_as_OT.lt_not_eq.
-  Defined.
-
-  Global Instance N_comp: Comparable N.
-  Proof.
-    constructor.
-    apply N_as_OT.compare.
-  Defined.
 
   Global Instance N_eqbtype : EqbType N :=
     {| eqb := N.eqb; eqb_spec := N.eqb_eq |}.
@@ -339,11 +133,8 @@ Section N.
 
   Global Instance N_compdec : CompDec N := {|
     Eqb := N_eqbtype;
-    Ordered := N_ord;
-    Comp := N_comp;
     Inh := N_inh
   |}.
-
 
 End N.
 
@@ -351,64 +142,6 @@ End N.
 Section BV.
 
   Import BITVECTOR_LIST.
-
-
-  Global Instance BV_ord n : OrdType (bitvector n).
-  Proof.
-    exists (fun a b => (bv_ult a b)).
-    unfold bv_ult, RAWBITVECTOR_LIST.bv_ult.
-    intros x y z; destruct x, y, z.
-    simpl. rewrite wf0, wf1, wf2. rewrite N.eqb_refl. simpl.
-    apply RAWBITVECTOR_LIST.ult_list_trans.
-    intros x y; destruct x, y.
-    simpl.
-    intros. unfold not.
-    intros. rewrite H0 in H.
-    unfold bv_ult, bv in *.
-    unfold RAWBITVECTOR_LIST.bv_ult, RAWBITVECTOR_LIST.size in H.
-    rewrite N.eqb_refl in H.
-    apply RAWBITVECTOR_LIST.ult_list_not_eq in H.
-    apply H. easy.
-  Defined.
-
-
-  Global Instance BV_comp n: Comparable (bitvector n).
-  Proof.
-    constructor.
-    intros x y.
-    case_eq (bv_ult x y).
-    intros.
-    apply OrderedType.LT.
-    unfold lt, BV_ord. auto.
-    case_eq (bv_eq x y).
-    intros.
-    apply OrderedType.EQ.
-    apply bv_eq_reflect. auto.
-    intros.
-    apply OrderedType.GT.
-    unfold lt, BV_ord. auto.
-    destruct (BV_ord n).
-    unfold bv_ult.
-    unfold bv_eq, RAWBITVECTOR_LIST.bv_eq,
-    RAWBITVECTOR_LIST.bits in H.
-    unfold bv_ult, RAWBITVECTOR_LIST.bv_ult in H0.
-    unfold is_true.
-
-    unfold RAWBITVECTOR_LIST.bv_ult, RAWBITVECTOR_LIST.size.
-    destruct x, y. simpl in *.
-    unfold RAWBITVECTOR_LIST.size in *.
-    rewrite wf0, wf1 in *.
-    rewrite N.eqb_refl in *.
-
-    apply RAWBITVECTOR_LIST.nlt_be_neq_gt.
-    rewrite !List.length_rev.
-    apply (f_equal (N.to_nat)) in wf0.
-    apply (f_equal (N.to_nat)) in wf1.
-    rewrite Nnat.Nat2N.id in wf0, wf1.
-    now rewrite wf0, wf1.
-    unfold RAWBITVECTOR_LIST.ult_list in H0. easy.
-    now apply RAWBITVECTOR_LIST.rev_neq in H.
-  Defined.
 
   Global Instance BV_eqbtype n : EqbType (bitvector n) :=
     {| eqb := @bv_eq n;
@@ -419,235 +152,31 @@ Section BV.
   Global Instance BV_inh n : Inhabited (bitvector n) :=
     {| default_value := zeros n |}.
 
-
   Global Instance BV_compdec n: CompDec (bitvector n) := {|
     Eqb := BV_eqbtype n;
-    Ordered := BV_ord n;
-    Comp := BV_comp n;
     Inh := BV_inh n
   |}.
 
 End BV.
 
 
-
-Section FArray.
-
-  Global Instance FArray_ord key elt
-           `{key_ord: OrdType key}
-           `{elt_ord: OrdType elt}
-           `{elt_inh: Inhabited elt}
-           `{key_comp: @Comparable key key_ord} : OrdType (farray key elt).
-  Proof.
-    exists (@lt_farray key elt key_ord key_comp elt_ord elt_inh).
-    apply lt_farray_trans.
-    unfold not.
-    intros.
-    apply lt_farray_not_eq in H.
-    apply H.
-    rewrite H0.
-    apply eqfarray_refl.
-  Defined.
-
-
-  Global Instance FArray_comp key elt
-           `{key_ord: OrdType key}
-           `{elt_ord: OrdType elt}
-           `{key_comp: @Comparable key key_ord}
-           `{elt_inh: Inhabited elt}
-           `{elt_comp: @Comparable elt elt_ord} : Comparable (farray key elt).
-  Proof.
-    constructor.
-    intros.
-    destruct (compare_farray key_comp elt_comp x y).
-    - apply OrderedType.LT. auto.
-    - apply OrderedType.EQ.
-      specialize (@eq_equal key elt key_ord key_comp elt_ord elt_comp elt_inh x y).
-      intros.
-      apply H in e.
-      now apply equal_eq in e.
-    - apply OrderedType.GT. auto.
-  Defined.
-
-  Global Instance FArray_eqbtype key elt
-           `{key_ord: OrdType key}
-           `{elt_ord: OrdType elt}
-           `{elt_eqbtype: EqbType elt}
-           `{key_comp: @Comparable key key_ord}
-           `{elt_comp: @Comparable elt elt_ord}
-           `{elt_inh: Inhabited elt}
-    : EqbType (farray key elt).
-  Proof.
-    exists FArray.equal.
-    intros.
-    split.
-    apply FArray.equal_eq.
-    intros. subst. apply eq_equal. apply eqfarray_refl.
-  Defined.
-
-  Global Instance FArray_dec key elt
-           `{key_ord: OrdType key}
-           `{elt_ord: OrdType elt}
-           `{elt_eqbtype: EqbType elt}
-           `{key_comp: @Comparable key key_ord}
-           `{elt_comp: @Comparable elt elt_ord}
-           `{elt_inh: Inhabited elt}
-    : DecType (farray key elt) := EqbToDecType.
-
-  Global Instance FArray_inh key elt
-           `{key_ord: OrdType key}
-           `{elt_inh: Inhabited elt} : Inhabited (farray key elt) :=
-    {| default_value := FArray.empty key_ord elt_inh |}.
-
-
-  Global Instance FArray_compdec key elt
-          `{key_compdec: CompDec key}
-          `{elt_compdec: CompDec elt} :
-    CompDec (farray key elt) :=
-    {|
-      Eqb := FArray_eqbtype key elt;
-      Ordered := FArray_ord key elt;
-      Comp := FArray_comp key elt ;
-      Inh := FArray_inh key elt
-    |}.
-
-End FArray.
-
-
 Section Uint63.
 
   Local Open Scope uint63_scope.
-
-  Let int_lt x y :=
-    if x <? y then True else False.
-
-  Global Instance int63_ord : OrdType int.
-  Proof.
-    exists int_lt; unfold int_lt.
-    - intros x y z.
-      case_eq (x <? y); intro;
-        case_eq (y <? z); intro;
-          case_eq (x <? z); intro;
-            simpl; try easy.
-      contradict H1.
-      rewrite not_false_iff_true.
-      rewrite ltb_spec in *.
-      exact (Z.lt_trans _ _ _ H H0).
-    - intros x y.
-      case_eq (x <? y); intro; simpl; try easy.
-      intros.
-      rewrite ltb_spec in *.
-      rewrite <- Misc.to_Z_eq.
-      exact (Z.lt_neq _ _ H).
-  Defined.
-
-
-  Global Instance int63_comp: Comparable int.
-  Proof.
-    constructor.
-    intros x y.
-    case_eq (x <? y); intro;
-      case_eq (x =? y); intro; unfold lt in *; simpl.
-    - rewrite Uint63.eqb_spec in H0.
-      contradict H0.
-      assert (int_lt x y). unfold int_lt.
-      rewrite H; trivial.
-      remember lt_not_eq. unfold lt in *. simpl in n.
-      exact (n _ _ H0).
-    - apply LT. unfold int_lt. rewrite H; trivial.
-    - apply EQ. rewrite Uint63.eqb_spec in H0; trivial.
-    - apply GT. unfold int_lt.
-      case_eq (y <? x); intro; simpl; try easy.
-      specialize (Misc.leb_ltb_eqb x y); intro.
-      contradict H2.
-      rewrite Misc.leb_negb_gtb. rewrite H1. simpl.
-      red. intro. symmetry in H2.
-      rewrite orb_true_iff in H2. destruct H2; contradict H2.
-      rewrite H. auto.
-      rewrite H0. auto.
-  Defined.
 
   Global Instance int63_eqbtype : EqbType int :=
     {| eqb := Uint63.eqb; eqb_spec := Uint63.eqb_spec |}.
 
   Global Instance int63_dec : DecType int := EqbToDecType.
 
-
   Global Instance int63_inh : Inhabited int := {| default_value := 0 |}.
 
   Global Instance int63_compdec : CompDec int := {|
     Eqb := int63_eqbtype;
-    Ordered := int63_ord;
-    Comp := int63_comp;
     Inh := int63_inh
   |}.
 
 End Uint63.
-
-
-Section option.
-
-  Generalizable Variable A.
-  Context `{HA : CompDec A}.
-
-
-  Definition option_lt (x y : option A) : Prop :=
-    match x, y with
-    | Some a, Some b => lt a b
-    | Some _, None => True
-    | None, Some _ => False
-    | None, None => False
-    end.
-
-
-  Lemma option_lt_trans : forall (x y z : option A),
-      option_lt x y -> option_lt y z -> option_lt x z.
-  Proof.
-    intros [a| ] [b| ] [c| ]; simpl; auto.
-    - apply lt_trans.
-    - intros _ [].
-  Qed.
-
-
-  Lemma option_lt_not_eq : forall (x y : option A), option_lt x y -> x <> y.
-  Proof.
-    intros [a| ] [b| ]; simpl; auto.
-    - intros H1 H2. inversion H2 as [H3]. revert H3. now apply lt_not_eq.
-    - discriminate.
-  Qed.
-
-
-  Global Instance option_ord : OrdType (option A) :=
-    Build_OrdType _ _ option_lt_trans option_lt_not_eq.
-
-
-  Definition option_compare : forall (x y : option A), Compare option_lt Logic.eq x y.
-  Proof.
-    intros [a| ] [b| ]; simpl.
-    - case_eq (compare a b); intros l H.
-      + now apply LT.
-      + apply EQ. now subst b.
-      + now apply GT.
-    - now apply LT.
-    - now apply GT.
-    - now apply EQ.
-  Defined.
-
-  Global Instance option_comp : Comparable (option A) := Build_Comparable _ _ option_compare.
-
-  Global Instance option_eqbtype : EqbType (option A) := Comparable2EqbType.
-
-
-  Global Instance option_inh : Inhabited (option A) := Build_Inhabited _ None.
-
-
-  Global Instance option_compdec : CompDec (option A) := {|
-    Ordered := option_ord;
-    Comp := option_comp;
-    Inh := option_inh
-  |}.
-
-End option.
 
 
 Section list.
@@ -656,71 +185,33 @@ Section list.
   Context `{HA : CompDec A}.
 
 
-  Fixpoint list_lt (xs ys : list A) : Prop :=
+  Fixpoint eqb_list (xs ys:list A) : bool :=
     match xs, ys with
-    | nil, nil => False
-    | nil, _::_ => True
-    | _::_, nil => False
-    | x::xs, y::ys => (lt x y) \/ (eqb x y /\ list_lt xs ys)
+    | nil, nil => true
+    | x::xs, y::ys => eqb x y && eqb_list xs ys
+    | _, _ => false
     end.
 
 
-  Definition list_compare : forall (x y : list A), Compare list_lt Logic.eq x y.
+  Lemma eqb_list_spec xs : forall ys, eqb_list xs ys = true <-> xs = ys.
   Proof.
-    induction x as [ |x xs IHxs]; intros [ |y ys]; simpl.
-    - now apply EQ.
-    - now apply LT.
-    - now apply GT.
-    - case_eq (compare x y); intros l H.
-      + apply LT. simpl. now left.
-      + case_eq (IHxs ys); intros l1 H1.
-        * apply LT. simpl. right. split; auto. now apply eqb_spec.
-        * apply EQ. now rewrite l, l1.
-        * apply GT. simpl. right. split; auto. now apply eqb_spec.
-      + apply GT. simpl. now left.
-  Defined.
-
-
-  Lemma list_lt_trans : forall (x y z : list A),
-      list_lt x y -> list_lt y z -> list_lt x z.
-  Proof.
-    induction x as [ |x xs IHxs]; intros [ |y ys] [ |z zs]; simpl; auto.
-    - inversion 1.
-    - intros [H1|[H1a H1b]] [H2|[H2a H2b]].
-      + left; eapply lt_trans; eauto.
-      + left. unfold is_true in H2a. rewrite eqb_spec in H2a. now subst z.
-      + left. unfold is_true in H1a. rewrite eqb_spec in H1a. now subst y.
-      + right. split.
-        * unfold is_true in H1a. rewrite eqb_spec in H1a. now subst y.
-        * eapply IHxs; eauto.
+    induction xs as [ |x xs IHxs]; intros [ |y ys]; split; simpl; intro H; auto; try discriminate.
+    - rewrite andb_true_iff in H. destruct H as [H1 H2].
+      rewrite eqb_spec in H1; subst.
+      now rewrite (IHxs ys) in H2; subst.
+    - injection H. intros -> ->. rewrite andb_true_iff; split.
+      + now rewrite eqb_spec.
+      + now rewrite IHxs.
   Qed.
 
-
-  Lemma list_lt_not_eq : forall (x y : list A), list_lt x y -> x <> y.
-  Proof.
-    induction x as [ |x xs IHxs]; intros [ |y ys]; simpl; auto.
-    - discriminate.
-    - intros [H1|[H1 H2]]; intros H; inversion H; subst.
-      + now apply (lt_not_eq _ _ H1).
-      + now apply (IHxs _ H2).
-  Qed.
-
-
-  Global Instance list_ord : OrdType (list A) :=
-    Build_OrdType _ _ list_lt_trans list_lt_not_eq.
-
-
-  Global Instance list_comp : Comparable (list A) := Build_Comparable _ _ list_compare.
-
-  Global Instance list_eqbtype : EqbType (list A) := Comparable2EqbType.
-
+  Global Instance list_eqbtype : EqbType (list A) :=
+    {| eqb := eqb_list;
+       eqb_spec := eqb_list_spec |}.
 
   Global Instance list_inh : Inhabited (list A) := Build_Inhabited _ nil.
 
-
   Global Instance list_compdec : CompDec (list A) := {|
-    Ordered := list_ord;
-    Comp := list_comp;
+    Eqb := list_eqbtype;
     Inh := list_inh
   |}.
 
@@ -732,66 +223,108 @@ Section prod.
   Generalizable Variables A B.
   Context `{HA : CompDec A} `{HB : CompDec B}.
 
+  Definition eqb_prod (x y:A * B) : bool :=
+    let (xa, xb) := x in
+    let (ya, yb) := y in
+    eqb xa ya && eqb xb yb.
 
-  Definition prod_lt (x y:A*B) : Prop :=
-    let (a1, b1) := x in
-    let (a2, b2) := y in
-    (lt a1 a2) \/ ((a1 = a2) /\ (lt b1 b2)).
-
-
-  Definition prod_compare : forall (x y:A*B), Compare prod_lt Logic.eq x y.
+  Lemma eqb_prod_spec : forall x y, eqb_prod x y = true <-> x = y.
   Proof.
-    intros [a1 b1] [a2 b2].
-    case_eq (compare a1 a2); intros l H.
-    - apply LT. simpl. now left.
-    - case_eq (compare b1 b2); intros l1 H1.
-      + apply LT. simpl. now right.
-      + apply EQ. now subst.
-      + apply GT. simpl. now right.
-    - apply GT. simpl. now left.
-  Defined.
-
-
-  Lemma prod_lt_trans : forall (x y z:A*B),
-      prod_lt x y -> prod_lt y z -> prod_lt x z.
-  Proof.
-    intros [a1 b1] [a2 b2] [a3 b3]; simpl.
-    intros [H1|[H1 H4]] [H2|[H2 H3]].
-    - left. eapply lt_trans; eauto.
-    - subst a3. now left.
-    - subst a2. now left.
-    - subst a2 a3. right. split; auto. eapply lt_trans; eauto.
+    intros [xa xb] [ya yb]; simpl; split; rewrite andb_true_iff.
+    - rewrite !eqb_spec. now intros [-> ->].
+    - intro H. rewrite !eqb_spec. now inversion H.
   Qed.
 
-
-  Lemma prod_lt_not_eq : forall (x y:A*B), prod_lt x y -> x <> y.
-  Proof.
-    intros [a1 b1] [a2 b2]; simpl.
-    intros [H1|[_ H1]] H3; inversion H3 as [[H4 H5]]; clear H3; subst a2 b2;
-      now apply (lt_not_eq _ _ H1).
-  Qed.
-
-
-  Global Instance prod_ord : OrdType (prod A B) :=
-    Build_OrdType _ _ prod_lt_trans prod_lt_not_eq.
-
-
-  Global Instance prod_comp : Comparable (prod A B) := Build_Comparable _ _ prod_compare.
-
-  Global Instance prod_eqbtype : EqbType (prod A B) := Comparable2EqbType.
-
+  Global Instance prod_eqbtype : EqbType (prod A B) :=
+    {| eqb := eqb_prod;
+       eqb_spec := eqb_prod_spec |}.
 
   Global Instance prod_inh : Inhabited (prod A B) :=
     Build_Inhabited _ (default_value, default_value).
 
-
   Global Instance prod_compdec : CompDec (prod A B) := {|
-    Ordered := prod_ord;
-    Comp := prod_comp;
+    Eqb := prod_eqbtype;
     Inh := prod_inh
   |}.
 
 End prod.
+
+
+Section option.
+
+  Generalizable Variable A.
+  Context `{HA : CompDec A}.
+
+  Definition eqb_option (x y:option A) : bool :=
+    match x, y with
+    | Some a, Some b => eqb a b
+    | None, None => true
+    | _, _ => false
+    end.
+
+  Lemma eqb_option_spec : forall x y, eqb_option x y = true <-> x = y.
+  Proof.
+    intros [a| ] [b| ]; simpl; split; try discriminate; try reflexivity; rewrite eqb_spec.
+    - now intros ->.
+    - intro H; now inversion H.
+  Qed.
+
+  Global Instance option_eqbtype : EqbType (option A) :=
+    {| eqb := eqb_option;
+       eqb_spec := eqb_option_spec |}.
+
+  Global Instance option_inh : Inhabited (option A) := Build_Inhabited _ None.
+
+  Global Instance option_compdec : CompDec (option A) := {|
+    Eqb := option_eqbtype;
+    Inh := option_inh
+  |}.
+
+End option.
+
+
+Section FArray.
+
+  Generalizable Variables key elt.
+  Context `{Hk : CompDec key}.
+  Context `{He : CompDec elt}.
+
+  Instance key_dec : DecType key := EqbToDecType.
+  Instance elt_dec : DecType elt := EqbToDecType.
+
+  Definition eqb_farray (a1 a2:farray key elt) : bool :=
+    let (l1, _, _) := a1 in
+    let (l2, _, _) := a2 in
+    eqb_list l1 l2.
+
+  From Stdlib Require Import ProofIrrelevance. (* TODO: remove *)
+
+  Lemma eqb_farray_spec : forall a1 a2, eqb_farray a1 a2 = true <-> a1 = a2.
+  Proof.
+    intros [athis aNoDup anodefault] [bthis bNoDup bnodefault]; simpl.
+    rewrite eqb_list_spec. split.
+    - intros ->. rewrite (proof_irrelevance _ aNoDup bNoDup).
+      now rewrite (proof_irrelevance _ anodefault bnodefault).
+    - intro H; now inversion H.
+  Qed.
+
+  Global Instance FArray_eqbtype : EqbType (farray key elt) :=
+    {| eqb := eqb_farray;
+       eqb_spec := eqb_farray_spec |}.
+
+  Global Instance FArray_dec : DecType (farray key elt) := EqbToDecType.
+
+  Global Instance FArray_inh : Inhabited (farray key elt) :=
+    {| default_value := @FArray.empty key elt _ |}.
+
+
+  Global Instance FArray_compdec : CompDec (farray key elt) :=
+    {|
+      Eqb := FArray_eqbtype;
+      Inh := FArray_inh
+    |}.
+
+End FArray.
 
 
 (* Register constants for OCaml access *)
